Netlist dsl

cava/Cava/Netlist.v
@@ -25,6 +25,7 @@ From Coq Require Import Ascii String.
 From Coq Require Import ZArith.
 From Coq Require Import Lists.List.
 From Coq Require Import Vector.
+From Coq Require Import Numbers.NaryFunctions.
 Import ListNotations.
 
 (******************************************************************************)
@@ -102,3 +103,137 @@ Definition initStateFrom (startAt : N) : CavaState
 
 Definition initState : CavaState
   := initStateFrom 2.
+
+
+
+Section Netlang.
+  Inductive type :=
+  | Hole : type
+  | Prim : type
+  | Mod  : type
+  | PortDecl: type
+  | List : type -> type
+  | Func : type -> type -> type.
+
+  Variable var: type ->  Type.
+
+  Inductive term : type -> Type :=
+  | Const : N -> term Hole
+  | Var : forall x, var x -> term x
+  | Abs : forall x y, (var x -> term y) -> term (Func x y)
+  | App : forall x y, term (Func x y) -> term x -> term y
+
+  | Prim2 : (N -> N -> Primitive) -> term Hole -> term Hole -> term Prim
+  | Prim3 : (N -> N -> N -> Primitive) -> term Hole -> term Hole -> term Hole -> term Prim
+  | Prim4 : (N -> N -> N -> N -> Primitive) -> term Hole -> term Hole -> term Hole -> term Hole -> term Prim
+  | Prim': (list N -> Primitive) -> term (List Hole) -> term Prim
+
+  | LiftList : forall x, list (term x) -> term (List x)
+  | Module' : string -> term (List Prim) -> term (List PortDecl) -> term (List PortDecl) -> term Mod
+  | Port' : string -> term Hole -> term PortDecl.
+End Netlang.
+
+Arguments Var _ [x] _.
+Arguments Abs _ [x y] _.
+Arguments App _ [x y] _.
+
+Arguments Const [var].
+
+Arguments Prim2 [var].
+Arguments Prim3 [var].
+Arguments Prim4 [var].
+Arguments Prim' [var].
+
+Arguments LiftList [var x].
+Arguments Module' [var].
+Arguments Port' [var].
+
+Fixpoint denoteType t :=
+match t with
+| Hole => N
+| Prim => Primitive
+| Mod => Module
+| PortDecl => PortDeclaration
+| List t => list (denoteType t)
+| Func t1 t2 => denoteType t1 -> denoteType t2
+end.
+
+Fixpoint denoteTerm t (e: term denoteType t) : denoteType t :=
+let dt := denoteTerm in
+match e in term _ t return denoteType t with
+| Var _ x => x
+| Abs _ f => fun x => dt _ (f x)
+| App _ f x => (dt _ f) (dt _ x)
+| Const x => x
+| Prim2 p x y => p (dt _ x) (dt _ y)
+| Prim3 p x y z => p (dt _ x) (dt _ y) (dt _ z)
+| Prim4 p x y z w => p (dt _ x) (dt _ y) (dt _ z) (dt _ w)
+| Prim' p xs => p (dt _ xs)
+| LiftList xs => (List.map (dt _) xs)
+| Module' name nl is os => mkModule name (dt _ nl) (dt _ is) (dt _ os)
+| Port' name x => mkPort name (BitPort (dt _ x))
+end.
+
+Fixpoint substitute' var t (e: term (term var) t): term var t :=
+let r := substitute' in
+match e with
+| Var _ x => x
+| Abs _ f => Abs _ (fun x => r _ _ (f (Var _ x)))
+| App _ f x => App _ (r _ _ f) (r _ _ x)
+| Const x => Const x
+| Prim2 p x y => Prim2 p (r _ _ x)(r _ _ y)
+| Prim3 p x y z => Prim3 p (r _ _ x) (r _ _ y) (r _ _ z)
+| Prim4 p x y z w => Prim4 p (r _ _ x) (r _ _ y) (r _ _ z) (r _ _ w)
+| Prim' p xs => Prim' p (r _ _ xs)
+| LiftList xs => LiftList (List.map (r _ _) xs)
+| Module' name nl is os => Module' name (r _ _ nl) (r _ _ is) (r _ _ os)
+| Port' name x => Port' name (r _ _ x)
+end.
+
+Definition Term t := forall var, term var t.
+Definition Term1 t1 t2 := forall var, var t1 -> term var t2.
+
+Definition substitute t1 t2 (e1: Term1 t1 t2) (e2: Term t1) : Term t2 :=
+fun var => substitute' _ _ (e1 (term var) (e2 var)).
+
+(*
+Takes an `NaryFunction` `N ^^ n --> B`, that has n arguments of type N returning type B.
+Automatically applies incrementing values of N starting at a. 
+e.g. if f :  A ^^ n --> B
+then autoNumber' _ 0 5 f == f 0 1 2 3 4
+*)
+Fixpoint autoNumber' (B:Type) (a:N) n : (N^^n-->B) -> B :=
+ match n return (N^^n-->B) -> B with
+  | O => fun x => x
+  | S n => fun x => autoNumber' B (a+1) n (x a)
+ end.
+
+Fixpoint autoNumber n t (f: nfun N n t) : t :=
+autoNumber' t (2%N) n f.
+
+Fixpoint countHoles t :=
+match t with
+| Func Hole t2 => 1 + countHoles t2
+| _ => 0
+end.
+
+Fixpoint CountHoles var t (_: term var t) := countHoles t.
+
+(* a netlist only to demonstrate arbitrary connections, the circuit itself is meaningless *)
+Example example_netlist var
+:= Abs var (fun x => Abs _ (fun y => Abs _ (fun w => Abs _ (fun z =>
+LiftList
+[ Prim2 Buf (Var _ x) (Var _ x)
+; Prim2 Buf (Var _ x) (Var _ y)
+; Prim2 Buf (Var _ y) (Var _ x)
+; Prim2 Buf (Var _ y) (Var _ y)
+; Prim2 Not (Var _ z) (Var _ w)
+; Prim2 Not (Var _ y) (Var _ z)
+]
+)))).
+
+Example netlist_denote_then_apply := denoteTerm _ (example_netlist _) 2%N 3%N 4%N 5%N.
+Example netlist_autonumber := autoNumber 4 _ (denoteTerm _ (example_netlist _)).
+Example netlist_countholes_autonumber := 
+  let ex := (example_netlist _)
+  in autoNumber (CountHoles _ _ ex) _ (denoteTerm _ ex).
